MapFind.v
@@ -5,6 +5,27 @@ Require Import Coq.FSets.FSetFacts.
 Require Import Coq.FSets.FMapAVL.
 Require Import Coq.FSets.FMapFacts.
 Require Import Coq.Program.Equality.
+Require Import Lia.
+
+
+Require Import Coq.Setoids.Setoid.
+
+Definition equivalent (n m : nat) : Prop :=
+  n = m.
+
+#[export]
+Instance equiv_rel : Equivalence equivalent.
+Proof.
+  split.
+  - unfold Reflexive. intros n. reflexivity.
+  - unfold Symmetric. intros n m H. symmetry. assumption.
+  - unfold Transitive. intros n m p H1 H2. transitivity m; assumption.
+Qed.
+
+Definition nat_equiv_class (n : nat) : Type :=
+  { m : nat | equivalent n m }.
+
+
 
 Require Import Top0.Keys.
 Require Import Top0.Definitions.
@@ -15,36 +36,88 @@ Module STProofs := ST.Raw.Proofs.
 Module STMapP := FMapFacts.Facts ST.
 Module STMapProp := FMapFacts.Properties ST.
 
+Definition AddToMap :=
+  fun(k : nat * nat) (v : tau) (m : Sigma) => ST.add k v m.
+
 Definition Functional_Map_Union (stty1 stty2 : Sigma) : Sigma :=
-  let f := fun (k : nat * nat) (v : tau) (m : Sigma) => ST.add k v m
-  in ST.fold f stty1 stty2.
+  ST.fold AddToMap stty1 stty2.
 
+Lemma In_node_iff_fold:
+  forall k e t l d this this1 this2 is_bst is_bst0 is_bst1 is_bst2,
+    ST.Raw.MapsTo l d (ST.this (ST.fold AddToMap {| ST.this := this; ST.is_bst := is_bst |}
+       {| ST.this := ST.Raw.Node this1 k e this2 t; ST.is_bst := is_bst0 |}))  
+   <-> (ST.Raw.MapsTo l d (ST.this(ST.fold AddToMap {| ST.this := this; ST.is_bst := is_bst |}
+       {| ST.this := this1; ST.is_bst := is_bst1 |}))) \/
+       (ST.Raw.MapsTo l d (ST.this(ST.fold AddToMap {| ST.this := this; ST.is_bst := is_bst |}
+       {| ST.this := this2; ST.is_bst := is_bst2 |}))) \/
+       ( ST.Raw.MapsTo k e this /\ l = k /\ d=e).
+Admitted.
 
-Lemma fold_add_empty:
-  forall x e h is_bst is_bst0,
-    {| ST.this := ST.Raw.Node  (ST.Raw.Leaf tau) x e  (ST.Raw.Leaf tau) h; ST.is_bst := is_bst |} =
-      ST.add x e {| ST.this := ST.Raw.Leaf tau; ST.is_bst := is_bst0 |}.
-Proof.
-  intros.
-  unfold ST.add. unfold ST.Raw.add. simpl.
+Lemma MapsTo_fold_Leaf:
+  forall l d l0 x e r h is_bst is_bst0,
+    ST.Raw.MapsTo l d
+      (ST.this
+         (ST.fold AddToMap {| ST.this := ST.Raw.Node l0 x e r h; ST.is_bst := is_bst |}
+                  {| ST.this := ST.Raw.Leaf tau; ST.is_bst := is_bst0 |})) <->
+    ST.Raw.MapsTo l d (ST.Raw.Node l0 x e r h).
 Admitted.
   
+Lemma Functional_Map_Union_find_2:
+  forall (sttya sttyb: ST.t tau) (l : ST.key) (t' : tau),
+    ST.Raw.bst (ST.this sttya) ->
+    ST.Raw.bst (ST.this (ST.fold AddToMap sttya sttyb)) ->
+    ST.find (elt:=tau) l (Functional_Map_Union sttya sttyb) = ST.find (elt:=tau) l sttya.
+Proof.
+  intros.
+  unfold Functional_Map_Union.
+  apply STProofs.find_mapsto_equiv; auto. 
+  split; intro.
+  - destruct sttya. destruct sttyb. simpl. induction this0.
+     + inversion is_bst; subst.
+       * simpl in *. assumption.
+       * eapply MapsTo_fold_Leaf.
+         eauto.         
+     + eapply In_node_iff_fold in H1.
+       destruct H1 as [HA | [HB | HC]]. 
+       * eapply IHthis0_1.  admit.
+         eauto.
+       * eapply IHthis0_2. admit.
+         eauto.
+       * unfold AddToMap in HC. 
+         destruct HC as [HA' [HB' HC']].
+         subst.  assumption.
+  - destruct sttya. destruct sttyb. simpl. induction this0.
+    + inversion is_bst; subst.
+      * simpl in *. assumption.
+      * apply STProofs.lt_tree_not_in in H4.
+        apply STProofs.gt_tree_not_in in H5.
+        now apply MapsTo_fold_Leaf.        
+    + eapply In_node_iff_fold.
+      * left. apply IHthis0_1.
+        admit.
+Admitted.
 
+
+
+  
+
+                   
 Lemma Functional_Map_Union_find_1:
   forall sttya sttyb (l : ST.key) (t' : tau),
     ST.find (elt:=tau) l (Functional_Map_Union sttya sttyb) = ST.find (elt:=tau) l sttya.
 Proof.
   intros.
-  unfold Functional_Map_Union. (*ST.fold.*)
+  unfold Functional_Map_Union.
   destruct sttya. destruct sttyb. simpl. induction this0.
   - inversion is_bst; subst.
     + reflexivity. 
-    + replace (ST.fold (fun (k : nat * nat) (v : tau) (m : Sigma) => ST.add k v m)
+    + replace (ST.fold AddToMap
                        {| ST.this := ST.Raw.Node l0 x e r h; ST.is_bst := is_bst |}
                        {| ST.this := ST.Raw.Leaf tau; ST.is_bst := is_bst0 |})
         with ( {| ST.this := ST.Raw.Node l0 x e r h; ST.is_bst := is_bst |} ).
       * reflexivity.
-      * unfold ST.add, ST.Raw.add. unfold ST.fold, ST.Raw.fold. simpl.
+      * unfold ST.fold. rewrite STProofs.fold_1; simpl; auto.
+        unfold fold_left. unfold ST.Raw.elements. simpl.
         admit.
   - inversion is_bst0; subst.
     assert (
