Definitions.v
@@ -1065,3 +1065,4 @@ Proof.
           with conj _ (conj _ (conj _ F)) =>
                F (stty, rho, env, ctxt) end); eauto.
 Qed.
+
